messageInvariantPrototypes/lib/MonotonicityLibrary.dfy
@@ -1,0 +1,12 @@
+include "UtilitiesLibrary.dfy"
+
+module MonotonicityLibrary {
+  import opened UtilitiesLibrary
+
+  datatype WriteOnceOption<T> = WOSome(value:T) | WONone
+  {
+    ghost predicate SatisfiesWriteOnce(past: WriteOnceOption<T>) {
+      past.WOSome? ==> past == this
+    }
+  }
+}
